Update patterns "always" and "constrained_until"

Constrained_Until.thy
@@ -2,40 +2,41 @@ theory Constrained_Until
   imports Always
 begin
 
-definition constrained_until where "constrained_until s1 s t A1 A2 \<equiv>
+definition constrained_until where "constrained_until s s1 t A1 A2 \<equiv>
 toEnvNum s1 s \<ge> t \<longrightarrow>
-(\<exists> s3. toEnvP s3 \<and> substate s1 s3 \<and> substate s3 s \<and> toEnvNum s1 s3 \<le> t \<and> A2 s3 \<and>
-(\<forall> s2. toEnvP s2 \<and> substate s1 s2 \<and> substate s2 s3 \<and> s2 \<noteq> s3 \<longrightarrow> A1 s2))"
+(\<exists> r2. toEnvP r2 \<and> s1 \<le> r2 \<and> r2 \<le> s \<and> toEnvNum s1 r2 \<le> t \<and> A2 s r2 \<and>
+(\<forall> r1. toEnvP r1 \<and> s1 \<le> r1 \<and> r1 < r2 \<longrightarrow> A1 s r1))"
 
-definition constrained_until_inv where "constrained_until_inv s1 s t t1 A1 A2 \<equiv>
-(\<exists> s3. toEnvP s3 \<and> substate s1 s3 \<and> substate s3 s \<and> toEnvNum s1 s3 \<le> t \<and> A2 s3 \<and>
-(\<forall> s2. toEnvP s2 \<and> substate s1 s2 \<and> substate s2 s3 \<and> s2 \<noteq> s3 \<longrightarrow> A1 s2)) \<or>
-toEnvNum s1 s < t1 \<and>
-(\<forall> s2. toEnvP s2 \<and> substate s1 s2 \<and> substate s2 s \<longrightarrow> A1 s2)"
+definition constrained_until_inv where "constrained_until_inv s s1 t t1 A1' A2' \<equiv>
+(\<exists> r2. toEnvP r2 \<and> s1 \<le> r2 \<and> r2 \<le> s \<and> toEnvNum s1 r2 \<le> t \<and> A2' s r2 \<and>
+(\<forall> r1. toEnvP r1 \<and> s1 \<le> r1 \<and> r1 < r2 \<longrightarrow> A1' s r1)) \<or>
+toEnvNum s1 s < t1 s \<and>
+(\<forall> r1. toEnvP r1 \<and> s1 \<le> r1 \<and> r1 \<le> s \<longrightarrow> A1' s r1)"
 
-lemma constrained_until_rule: "
-consecutive s0 s \<Longrightarrow>
-(\<forall> s1. toEnvP s1 \<and>  substate s1 s0 \<and> A1 s1 \<longrightarrow> A1' s1) \<and>
-(\<forall> s1. toEnvP s1 \<and> substate s1 s0 \<and> A2 s1 \<longrightarrow> A2' s1) \<and>
- (t1 = 0 \<or> A2' s \<and> t1 \<le> t \<or> A1' s \<and> t1 < t1') \<Longrightarrow>
-\<forall> s1. toEnvP s1 \<and>  substate s1 s0 \<and> constrained_until_inv s1 s0 t t1 A1 A2 \<longrightarrow> constrained_until_inv s1 s t t1' A1' A2'"
-  apply(unfold constrained_until_inv_def)
+lemma constrained_until_rule[patternintro]: "
+consecutive s s' \<Longrightarrow>
+always_imp s (A1' s) (A1' s') \<and>
+always_imp s (A2' s) (A2' s') \<and>
+ (t1 s = 0 \<or> A2' s' s' \<and> t1 s \<le> t \<or> A1' s' s' \<and> t1 s < t1 s') \<Longrightarrow>
+always_imp s (\<lambda> s1. constrained_until_inv s s1 t t1 A1' A2') (\<lambda> s1. constrained_until_inv s' s1 t t1 A1' A2')"
+  apply(unfold constrained_until_inv_def always_imp_def)
+    unfolding less_eq_state.simps less_state.simps
   apply(rule allI)
   subgoal for s1
     apply(rule impI)
     apply(erule conjE)+
     apply(rotate_tac -1)
     apply(erule disjE)
-     apply (metis consecutive.elims(2) substate_trans)
+     apply (metis consecutive.simps substate_trans)
     apply(erule disjE)
      apply simp
     apply(erule disjE)
      apply(rule disjI1)
-     apply(rule exI[of _ s])
+     apply(rule exI[of _ s'])
      apply(rule conjI)
       apply simp
      apply(rule conjI)
-    apply simp
+      apply simp
       apply (meson substate_trans)
      apply(rule conjI)
       apply simp
@@ -48,73 +49,44 @@ consecutive s0 s \<Longrightarrow>
     by (smt (verit, ccfv_SIG) consecutive.elims(2) less_imp_add_positive less_numeral_extra(3) less_one linorder_neqE_nat nat_add_left_cancel_less substate_noteq_imp_substate_of_pred trans_less_add1 zero_less_one)
   done
 
-lemma constrained_until_einv2req: "
-(\<forall> s1. toEnvP s1 \<and>  substate s1 s \<and> A1 s1 \<longrightarrow> A1' s1) \<and>
-(\<forall> s1. toEnvP s1 \<and> substate s1 s \<and> A2 s1 \<longrightarrow> A2' s1) \<and>
-t1 \<le> t \<Longrightarrow>
-\<forall> s1. toEnvP s1 \<and>  substate s1 s \<and> constrained_until_inv s1 s t t1 A1 A2 \<longrightarrow> constrained_until s1 s t A1' A2'"
-  apply(unfold constrained_until_inv_def constrained_until_def)
+lemma constrained_until_einv2req[patternintro]: "
+always_imp s (A1' s) (A1 s) \<and>
+always_imp s (A2' s) (A2 s) \<and>
+t1 s \<le> t \<Longrightarrow>
+always_imp s (\<lambda> s1. constrained_until_inv s s1 t t1 A1' A2') (\<lambda> s1. constrained_until s s1 t A1 A2)"
+  unfolding constrained_until_inv_def constrained_until_def always_imp_def less_eq_state.simps less_state.simps
   by (metis dual_order.trans substate_trans verit_comp_simplify1(3))
 
-lemma constrained_until_one_point: "
-toEnvP s \<Longrightarrow>A2 s \<or> A1 s \<and> t1 > 0 \<Longrightarrow> constrained_until_inv s s t t1 A1 A2"
-  apply(unfold constrained_until_inv_def)
-  by (metis less_eq_nat.simps(1) substate_antisym substate_refl toEnvNum_id)
+lemma constrained_until_one_point[patternintro]: "
+toEnvP s \<Longrightarrow>A2' s s \<or> A1' s s \<and> t1 s > 0 \<Longrightarrow> constrained_until_inv s s t t1 A1' A2'"
+  unfolding constrained_until_inv_def always_imp_def
+  by (metis bot_nat_0.extremum dual_order.refl leD order_le_imp_less_or_eq toEnvNum_id)
 
-definition P1inv where "P1inv s t t1 A1 A3 A2 \<equiv> 
-always s (\<lambda> s1.  A1 s1 \<longrightarrow> constrained_until_inv s1 s t t1 A3 A2)"
+definition P1 where "P1 s t A1 A2 A3 \<equiv> 
+always s s (\<lambda> r2 r1.  \<not> A1 r1 \<or> constrained_until r2 r1 t A2 A3)"
 
-definition P1 where "P1 s t A1 A3 A2 \<equiv> 
-always s (\<lambda> s1.  A1 s1 \<longrightarrow> constrained_until s1 s t A3 A2)"
+definition P1_inv where "P1_inv s t t1 A1 A2' A3' \<equiv> 
+always_inv s (\<lambda> r2 r1.  \<not> A1 r1 \<or> constrained_until_inv r2 r1 t t1 A2' A3')"
 
-lemma P1'einv2req: "P1inv s t t1 A1 A2 A3 \<Longrightarrow> t1 \<le> t \<Longrightarrow> P1 s t A1 A2 A3"
-  apply(unfold P1inv_def P1_def)
-  using always_einv2req constrained_until_einv2req
-  by (smt (verit, ccfv_SIG))
-
-lemma P1'inv_rule_gen: "
- P1inv s0 t t1 A1 A3 A2 \<Longrightarrow> consecutive s0 s \<Longrightarrow>
-(\<not> A1 s \<or> A2' s \<or> A3' s \<and> t2 > 0)  \<and>
-(\<forall> s1. toEnvP s1 \<and> substate s1 s0 \<and> A3 s1 \<longrightarrow> A3' s1) \<and> (\<forall> s1. toEnvP s1 \<and> substate s1 s0 \<and> A2 s1 \<longrightarrow> A2' s1) \<and>  (t1 = 0 \<or> A2' s \<and> t1 \<le> t \<or> A3' s \<and> t1 < t2) \<Longrightarrow>
- P1inv s t t2 A1 A3' A2'"
-  apply(unfold P1inv_def)
-  apply(simp only: imp_conv_disj)
-  apply(erule always_rule)
-  apply simp
-   apply(erule conjE)
+schematic_goal P1'inv_rule_gen: "
+ P1_inv s t t1 A1 A2' A3' \<Longrightarrow> consecutive s s' \<Longrightarrow>
+B1 \<and> B2 \<Longrightarrow>
+ P1_inv s' t t1 A1 A2' A3'"
+  unfolding P1_inv_def
+  apply(erule elims)
+   apply assumption
+  apply(erule conjE)
   subgoal premises prems1
     apply(rule conjI)
      apply(insert prems1(1,2))[1]
-     apply(erule disjE)
-      apply(rule disjI1)
-      apply assumption (*apply simp*)
-     apply(rule disjI2)
-     apply(rule constrained_until_one_point)
-      apply simp
-     apply assumption (*apply simp*)
-    apply(insert prems1(1,3))[1]
-    apply(rule all_disj_rule)
-    apply(rule conjI)
-     apply simp
-    apply(rule constrained_until_rule)
-     apply simp
-    apply simp
-    done
-  done
-
-lemma P1'inv_rule: "
- P1inv s0 t t1 A1 A3 A2 \<Longrightarrow> consecutive s0 s \<Longrightarrow>
-(\<not> A1 s \<or> A2 s \<or> A3 s \<and> t2 > 0)  \<and>
-(t1 = 0 \<or> A2 s \<and> t1 \<le> t \<or> A3 s \<and> t1 < t2) \<Longrightarrow>
- P1inv s t t2 A1 A3 A2"
-  using P1'inv_rule_gen by simp
-
-lemma P1'einv2req_gen: "P1inv s t t1 A1 A2 A3 \<Longrightarrow> (\<forall> s1. toEnvP s1 \<and> substate s1 s \<and> A2 s1 \<longrightarrow> A2' s1) \<and> (\<forall> s1. toEnvP s1 \<and> substate s1 s \<and> A3 s1 \<longrightarrow> A3' s1) \<and>
- t1 \<le> t \<Longrightarrow> P1 s t A1 A2' A3'"
-  apply(unfold P1inv_def P1_def)
-  using always_einv2req constrained_until_einv2req
-  by (smt (verit, ccfv_SIG))
-
-end
 
 
+
+
+
+
+
+
+
+
+ 
